Restart refinements folder

rupicola/refinements/EquivRel.fsti
@@ -9,21 +9,21 @@ open SyntacticTypes
 
 (** Cross Language Binary Logical Relation between F* and STLC expressions
      for __closed terms__. **)
-let rec (∋) (t:typ) (p:elab_typ t * closed_exp) : Tot Type0 (decreases %[t;0]) =
+let rec (∋) (t:typsr) (p:get_Type t * closed_exp) : Tot Type0 (decreases %[get_rel t;0]) =
   let fs_v = fst p in
   let e = snd p in
-  match t with
-  | TUnit -> fs_v == () /\ e == EUnit
-  | TBool -> (fs_v == true /\ e == ETrue) \/ (fs_v == false /\ e == EFalse)
-  | TArr t1 t2 -> begin
-    let fs_f : elab_typ t1 -> elab_typ t2 = fs_v in
+  match get_rel t with
+  | RUnit -> fs_v == () /\ e == EUnit
+  | RBool -> (fs_v == true /\ e == ETrue) \/ (fs_v == false /\ e == EFalse)
+  | RArr #t1 #t2 #s1 #s2 r1 r2 -> begin
+    let fs_f : s1 -> s2 = fs_v in
     match e with
     | ELam e' ->
-      (forall (v:value) (fs_v:elab_typ t1). t1 ∋ (fs_v, v) ==>
-        t2 ⦂ (fs_f fs_v, subst_beta v e'))
+      (forall (v:value) (fs_v:s1). (| _, _, r1 |) ∋ (fs_v, v) ==>
+        (| _, _, r2 |) ⦂ (fs_f fs_v, subst_beta v e'))
     | _ -> False
   end
-and (⦂) (t:typ) (p: elab_typ t * closed_exp) : Tot Type0 (decreases %[t;1]) =
+and (⦂) (t:typsr) (p: get_Type t * closed_exp) : Tot Type0 (decreases %[get_rel t;1]) =
   let fs_e = fst p in
   let e = snd p in
   forall (e':closed_exp). steps e e' ==> irred e' ==> t ∋ (fs_e, e')
@@ -50,11 +50,11 @@ let lem_values_are_expressions t fs_e e : (** lemma used by Amal **)
 
 val fs_env (g:env) : Type u#0
 val fs_empty : fs_env empty
-val get_v : #g:env -> fs_env g -> x:var{Some? (g x)} -> elab_typ (Some?.v (g x))
-val fs_extend : #g:env -> fs_s:fs_env g -> #t:typ -> elab_typ t -> fs_env (extend t g)
-val fs_shrink : #t:typ -> #g:env -> fs_env (extend t g) -> fs_env g
+val get_v : #g:env -> fs_env g -> x:var{Some? (g x)} -> get_Type (Some?.v (g x))
+val fs_extend : #g:env -> fs_s:fs_env g -> #t:typsr -> get_Type t -> fs_env (extend t g)
+val fs_shrink : #t:typsr -> #g:env -> fs_env (extend t g) -> fs_env g
 
-val lem_fs_extend #g (fs_s:fs_env g) #t (v:elab_typ t) : Lemma (
+val lem_fs_extend #g (fs_s:fs_env g) #t (v:get_Type t) : Lemma (
   (forall (x:var). Some? (g x) ==>  get_v fs_s x == get_v (fs_extend fs_s v) (x+1)) /\
   get_v (fs_extend fs_s v) 0 == v)
   [SMTPat (fs_extend fs_s v)]
@@ -63,7 +63,7 @@ val lem_fs_shrink #g #t (fs_s:fs_env (extend t g)) : Lemma (
   (forall (x:var). Some? (g x) ==>  get_v fs_s (x+1) == get_v (fs_shrink fs_s) x))
   [SMTPat (fs_shrink fs_s)]
 
-val shrink_extend_inverse #g (fs_s:fs_env g) #t (x:elab_typ t) : Lemma (fs_shrink (fs_extend fs_s x) == fs_s)
+val shrink_extend_inverse #g (fs_s:fs_env g) #t (x:get_Type t) : Lemma (fs_shrink (fs_extend fs_s x) == fs_s)
   [SMTPat (fs_shrink (fs_extend fs_s x))]
 
 let (∽) (#g:env) #b (s:gsub g b) (fs_s:fs_env g) : Type0 =
@@ -72,16 +72,16 @@ let (∽) (#g:env) #b (s:gsub g b) (fs_s:fs_env g) : Type0 =
 
 (** Cross Language Binary Logical Relation between F* and STLC expressions
      for __open terms__. **)
-let equiv (#g:env) (t:typ) (fs_e:fs_env g -> elab_typ t) (e:exp) : Type0 =
+let equiv (#g:env) (t:typsr) (fs_e:fs_env g -> get_Type t) (e:exp) : Type0 =
   fv_in_env g e /\
   forall b (s:gsub g b) (fs_s:fs_env g).
     s ∽ fs_s ==>  t ⦂ (fs_e fs_s, gsubst s e)
 
-let (≈) (#g:env) (#t:typ) (fs_v:fs_env g -> elab_typ t) (e:exp) : Type0 =
+let (≈) (#g:env) (#t:typsr) (fs_v:fs_env g -> get_Type t) (e:exp) : Type0 =
   equiv #g t fs_v e
 
 (** Equiv closed terms **)
-let equiv_closed_terms (#t:typ) (fs_e:elab_typ t) (e:closed_exp) :
+let equiv_closed_terms (#t:typsr) (fs_e:get_Type t) (e:closed_exp) :
   Lemma (requires equiv #empty t (fun _ -> fs_e) e)
         (ensures  t ⦂ (fs_e, e)) =
   eliminate forall b (s:gsub empty b) (fs_s:fs_env empty).
@@ -89,34 +89,40 @@ let equiv_closed_terms (#t:typ) (fs_e:elab_typ t) (e:closed_exp) :
 
 (** Rules **)
 
+let tunit : typsr =
+  (| _, _, RUnit |)
+
 let equiv_unit g
-  : Lemma ((fun (_:fs_env g) -> ()) `equiv TUnit` EUnit)
-  = assert ((fun (_:fs_env g) -> ()) `equiv TUnit` EUnit) by (explode ())
+  : Lemma ((fun (_:fs_env g) -> ()) `equiv tunit` EUnit)
+  = assert ((fun (_:fs_env g) -> ()) `equiv tunit` EUnit) by (explode ())
+
+let tbool : typsr =
+  (| _, _, RBool |)
 
 let equiv_true g
-  : Lemma ((fun (_:fs_env g) -> true) `equiv TBool` ETrue)
-  = assert ((fun (_:fs_env g) -> true) `equiv TBool` ETrue) by (explode ())
+  : Lemma ((fun (_:fs_env g) -> true) `equiv tbool` ETrue)
+  = assert ((fun (_:fs_env g) -> true) `equiv tbool` ETrue) by (explode ())
 
 let equiv_false g
-  : Lemma ((fun (_:fs_env g) -> false) `equiv TBool` EFalse)
-  = assert ((fun (_:fs_env g) -> false) `equiv TBool` EFalse) by (explode ())
+  : Lemma ((fun (_:fs_env g) -> false) `equiv tbool` EFalse)
+  = assert ((fun (_:fs_env g) -> false) `equiv tbool` EFalse) by (explode ())
 
 let equiv_var g (x:var{Some? (g x)})
   : Lemma ((fun (fs_s:fs_env g) -> get_v fs_s x) ≈ EVar x)
   = assert ((fun (fs_s:fs_env g) -> get_v fs_s x) ≈ EVar x) by (explode ())
 
-let equiv_lam g (t1:typ) (body:exp) (t2:typ) (f:fs_env g -> elab_typ (TArr t1 t2)) : Lemma
+let equiv_lam g (t1:typsr) (body:exp) (t2:typsr) (f:fs_env g -> get_Type (mk_arrow t1 t2)) : Lemma
   (requires (fun (fs_s:fs_env (extend t1 g)) -> f (fs_shrink #t1 fs_s) (get_v fs_s 0)) ≈ body)
             // the asymmetry is here. body is an open expression, while for f, I don't have an open expression
             // the equiv is quantifying over the free variable of body, but not get_v
   (ensures f ≈ (ELam body)) =
   lem_fv_in_env_lam g t1 body;
   let g' = extend t1 g in
-  introduce forall b (s:gsub g b) fs_s. s ∽ fs_s ==> TArr t1 t2 ⦂ (f fs_s, gsubst s (ELam body)) with begin
+  introduce forall b (s:gsub g b) fs_s. s ∽ fs_s ==> mk_arrow t1 t2 ⦂ (f fs_s, gsubst s (ELam body)) with begin
     introduce _ ==> _ with _. begin
       let body' = subst (sub_elam s) body in
       assert (gsubst s (ELam body) == ELam body');
-      introduce forall (v:value) (fs_v:elab_typ t1). t1 ∋ (fs_v, v) ==>  t2 ⦂ (f fs_s fs_v, subst_beta v body') with begin
+      introduce forall (v:value) (fs_v:get_Type t1). t1 ∋ (fs_v, v) ==>  t2 ⦂ (f fs_s fs_v, subst_beta v body') with begin
         introduce _ ==> _ with _. begin
           let s' = gsub_extend s t1 v in
           let fs_s' = fs_extend fs_s fs_v in
@@ -132,13 +138,13 @@ let equiv_lam g (t1:typ) (body:exp) (t2:typ) (f:fs_env g -> elab_typ (TArr t1 t2
           assert (t2 ⦂ (f fs_s fs_v, subst_beta v body'))
         end
       end;
-      assert (TArr t1 t2 ∋ (f fs_s, gsubst s (ELam body)));
-      lem_values_are_expressions (TArr t1 t2) (f fs_s) (gsubst s (ELam body));
-      assert (TArr t1 t2 ⦂ (f fs_s, gsubst s (ELam body)))
+      assert (mk_arrow t1 t2 ∋ (f fs_s, gsubst s (ELam body)));
+      lem_values_are_expressions (mk_arrow t1 t2) (f fs_s) (gsubst s (ELam body));
+      assert (mk_arrow t1 t2 ⦂ (f fs_s, gsubst s (ELam body)))
     end
   end
 
-let equiv_app g (t1:typ) (t2:typ) (e1:exp) (e2:exp) (fs_e1:fs_env g -> elab_typ (TArr t1 t2)) (fs_e2:fs_env g -> elab_typ t1) : Lemma
+let equiv_app g (t1:typsr) (t2:typsr) (e1:exp) (e2:exp) (fs_e1:fs_env g -> get_Type (mk_arrow t1 t2)) (fs_e2:fs_env g -> get_Type t1) : Lemma
   (requires fs_e1 ≈ e1 /\ fs_e2 ≈ e2)
   (ensures (fun fs_s -> (fs_e1 fs_s) (fs_e2 fs_s)) ≈ (EApp e1 e2)) =
   lem_fv_in_env_app g e1 e2;
@@ -152,7 +158,7 @@ let equiv_app g (t1:typ) (t2:typ) (e1:exp) (e2:exp) (fs_e1:fs_env g -> elab_typ 
           let steps_e_e' : squash (steps (EApp (gsubst s e1) (gsubst s e2)) e') = () in
           FStar.Squash.map_squash #_ #(squash (t2 ∋ (fs_e, e'))) steps_e_e' (fun steps_e_e' ->
             let (e11, e2') = destruct_steps_eapp (gsubst s e1) (gsubst s e2) e' steps_e_e' in
-            assert (TArr t1 t2 ∋ (fs_e1', ELam e11));
+            assert (mk_arrow t1 t2 ∋ (fs_e1', ELam e11));
             assert (t1 ∋ (fs_e2', e2'));
             assert (t2 ⦂ (fs_e, subst_beta e2' e11));
             assert (t2 ∋ (fs_e, e'))
@@ -162,7 +168,7 @@ let equiv_app g (t1:typ) (t2:typ) (e1:exp) (e2:exp) (fs_e1:fs_env g -> elab_typ 
     end
   end
 
-let equiv_if g (t:typ) (e1:exp) (e2:exp) (e3:exp) (fs_e1:fs_env g -> elab_typ TBool) (fs_e2:fs_env g -> elab_typ t) (fs_e3:fs_env g -> elab_typ t) : Lemma
+let equiv_if g (t:typsr) (e1:exp) (e2:exp) (e3:exp) (fs_e1:fs_env g -> get_Type tbool) (fs_e2:fs_env g -> get_Type t) (fs_e3:fs_env g -> get_Type t) : Lemma
   (requires fs_e1 ≈ e1 /\ fs_e2 ≈ e2 /\ fs_e3 ≈ e3)
   (ensures (fun fs_s -> if fs_e1 fs_s then fs_e2 fs_s else fs_e3 fs_s) ≈ EIf e1 e2 e3) =
   lem_fv_in_env_if g e1 e2 e3;
@@ -177,7 +183,7 @@ let equiv_if g (t:typ) (e1:exp) (e2:exp) (e3:exp) (fs_e1:fs_env g -> elab_typ TB
           let steps_e_e' : squash (steps (EIf (gsubst s e1) (gsubst s e2) (gsubst s e3)) e') = () in
           FStar.Squash.map_squash #_ #(squash (t ∋ (fs_e, e'))) steps_e_e' (fun steps_e_e' ->
             let e1' = destruct_steps_eif (gsubst s e1) (gsubst s e2) (gsubst s e3) e' steps_e_e' in
-            assert (TBool ∋ (fs_e1', e1'));
+            assert (tbool ∋ (fs_e1', e1'));
             assert (t ∋ (fs_e, e'))
           )
         end
